theories/simplang/simple_inv/adequacy.v
@@ -43,7 +43,7 @@ Proof.
   iSpecialize ("Hprog_rel" $! HΣ).
   iIntros "Hp_t Hp_s Hmt #Hgs_t #Hgs_s".
   iMod ("Hprog_rel" with "[//] [$] [$] [$] [$]") as "[#Hvs $]".
-  iMod (heap_bij_insert_globals with "Hbij Hmt Hvs") as (L') "[Hbij #Hls]"; [done| ].
+  iMod (heapbij_insert_globals with "Hbij Hmt Hvs") as (L') "[Hbij #Hls]"; [done| ].
   iModIntro. iSplitL "Hbij"; [|iSplitR; [done|]].
   - iExists _. iFrame. iExists _,_. by iFrame "#".
   - iIntros (??) "$".
